Qualifiers with tags added

Benchmarks/FluxRS/FibFibSlow.lean
@@ -1,23 +1,46 @@
+import Lean
 import LeanFixpoint
 
-noncomputable def fib_fib : Int → Int := sorry
-@[simp] axiom fib_base (n : Int) : n ≤ 1 → fib_fib n = 1
-@[simp] axiom fib_rec (n : Int) : n > 1 → fib_fib n = fib_fib (n-1) + fib_fib (n-2)
+open Lean Meta
+
+@[grind]
+def fib_spec_fib (n : Int) : Int :=
+  if n <= 1 then 1
+  else fib_spec_fib (n - 1) + fib_spec_fib (n - 2)
+  termination_by n.toNat
+
+@[qualif] def q_le          (a b : Int) : Prop := a ≤ b
+@[qualif] def q_gt_one      (v : Int)   : Prop := v > 1
+@[qualif] def q_eq_fib      (v i : Int) : Prop := v = fib_spec_fib i
+@[qualif] def q_eq_fib_pred (v i : Int) : Prop := v = fib_spec_fib (i - 1)
 
 def FibFibSlow :=
  ∀ (n₀ : Int),
   (n₀ ≥ 0) ->
    ((¬(n₀ ≤ 1)) ->
     (((n₀ - 1) ≥ 0)) ∧
-    (((fib_fib (n₀ - 1)) ≥ 0) ->
+    (((fib_spec_fib (n₀ - 1)) ≥ 0) ->
      (((n₀ - 2) ≥ 0)) ∧
-     (((fib_fib (n₀ - 2)) ≥ 0) ->
-      (((fib_fib (n₀ - 1)) + (fib_fib (n₀ - 2))) = (fib_fib n₀)))
+     (((fib_spec_fib (n₀ - 2)) ≥ 0) ->
+      (((fib_spec_fib (n₀ - 1)) + (fib_spec_fib (n₀ - 2))) = (fib_spec_fib n₀)))
      )
     ) ∧
    ((n₀ ≤ 1) ->
-    (1 = (fib_fib n₀)))
+    (1 = (fib_spec_fib n₀)))
 
 def FibFibSlow_proof : FibFibSlow := by
-  solve_fixpoint
-  
+  -- solve_fixpoint
+  sorry
+
+#eval show MetaM Unit from do
+  let qs ← getQualifiers
+  for q in qs do
+    let ty ← inferType q
+    let ci ← getConstInfo q.constName!
+    IO.println s!" {q} : {← ppExpr ty}"
+    if let some val := ci.value? then
+      IO.println s!"    = {← ppExpr val}"
+
+example (i n : Int)   :
+    (i + 1) ≤ n → fib_spec_fib i = fib_spec_fib ((i + 1) - 1) := by
+  grind
